Hs/HsTerm/Definition.lean
@@ -78,11 +78,11 @@ namespace HsTerm
  | HsVar _ => 0
  | HsName _ => 0
  | HsHole t1 => size t1 + 1
- | HsAnnotate _ t2 => size t2 + 1
+ | HsAnnotate t1 t2 => size t1 + size t2 + 1
  | HsCtor2 _ t1 t2 => size t1 + size t2 + 1
  | HsBind2 _ t1 t2 => size t1 + size t2 + 1
  | HsLet t1 t2 t3 => size t1 + size t2 + size t3 + 1
- | HsIte _ t1 t2 t3 => size t1 + size t2 + size t3 + 1
+ | HsIte t1 t2 t3 t4 => size t1 + size t2 + size t3 + size t4 + 1
 end HsTerm
 
 instance sizeOf_HsTerm : SizeOf HsTerm where
